compiler/backend/proofs/data_to_wordProofScript.sml
@@ -2070,11 +2070,12 @@ Proof
   simp[COND_RAND]>>
   fs[word_good_handlers_three_to_two_reg]>>
   match_mp_tac word_good_handlers_remove_dead>>
+  match_mp_tac word_cseProofTheory.word_good_handlers_word_common_subexp_elim >>
   simp[word_good_handlers_full_ssa_cc_trans,word_good_handlers_inst_select]>>
   match_mp_tac word_good_handlers_word_simp>>
   fs[FORALL_PROD]>>
   metis_tac[EL_MEM]
-QED;
+QED
 
 Theorem word_get_code_labels_word_to_word_incr_helper:
   ∀oracles.
@@ -2097,7 +2098,8 @@ Proof
     fs[COND_RAND]>>
     fs[word_get_code_labels_three_to_two_reg]>>
     old_drule (word_get_code_labels_remove_dead|>SIMP_RULE std_ss [SUBSET_DEF])>>
-    simp[word_get_code_labels_full_ssa_cc_trans,word_get_code_labels_inst_select]>>
+    simp[word_get_code_labels_full_ssa_cc_trans,word_get_code_labels_inst_select,
+         word_cseProofTheory.word_get_code_labels_word_common_subexp_elim]>>
     strip_tac>>
     old_drule (word_get_code_labels_word_simp|>SIMP_RULE std_ss [SUBSET_DEF])>>
     rw[]>>fs[FORALL_PROD,EXISTS_PROD,PULL_EXISTS,EVERY_MEM]>>
@@ -2170,7 +2172,7 @@ val word_get_code_labels_MemEqList = Q.prove(`
 Triviality part_to_words_isWord:
   ∀h c m i w ws.
     part_to_words c m h i = SOME (w,ws) ∧
-    (∀n v. lookup n m = SOME v ⇒ isWord (SND v)) ⇒
+    (∀n v. sptree$lookup n m = SOME v ⇒ isWord (SND v)) ⇒
     EVERY isWord (MAP SND ws) ∧ isWord (SND w)
 Proof
   Cases_on ‘h’ \\ fs [part_to_words_def] \\ rw []
@@ -2187,7 +2189,7 @@ QED
 Triviality parts_to_words_isWord:
   ∀ps c w ws m n i.
     parts_to_words c m n ps i = SOME (w,ws) ∧
-    (∀n v. lookup n m = SOME v ⇒ isWord (SND v)) ⇒
+    (∀n v. sptree$lookup n m = SOME v ⇒ isWord (SND v)) ⇒
     EVERY isWord (MAP SND ws) ∧ isWord (SND w)
 Proof
   Induct
